theories/Utils/Vectors.v
@@ -1,141 +1,151 @@
 From Coq Require Import
-  Lia.
+  Lia Nat VectorDef VectorEq ProofIrrelevance.
+Import VectorNotations EqNotations.
 From TinyRAM.Utils Require Import
-  Fin.
-From TinyRAM.Utils Require Import
-  Arith.
-Import PeanoNat.Nat.
-Require Import ProofIrrelevance.
-Require Import VectorDef.
-Import VectorNotations.
-Import EqNotations.
+  Fin Arith.
 
-Definition vector_length_coerce : forall {A n m},
-    n = m ->
-    Vector.t A n ->
-    Vector.t A m.
-  intros A n m eq v. rewrite <- eq. assumption. Defined.
+Import PeanoNat.Nat(succ_inj, 
+                    add_assoc, 
+                    add_comm, 
+                    nlt_0_r,
+                    mul_comm,
+                    ltb_lt).
 
-Theorem vector_length_coerce_trans : forall {A n m o}
-    (eq1 : n = m) (eq2 : m = o) (v : Vector.t A n),
-    (vector_length_coerce eq2 (vector_length_coerce eq1 v))
-    = (vector_length_coerce (eq_trans eq1 eq2) v).
+Theorem cast_rew : forall {A} {m n} (eq : m = n) (v : t A m),
+  cast v eq = rew eq in v.
+Proof.
+  intros A m n eq v. 
+  generalize dependent n; induction v; intros.
+  - destruct eq; reflexivity.
+  - destruct eq; simpl; rewrite IHv; reflexivity.
+Qed.
+
+Theorem cast_trans : forall {A n m o}
+    (eq1 : n = m) (eq2 : m = o) (v : t A n),
+    (cast (cast v eq1) eq2)
+    = (cast v (eq_trans eq1 eq2)).
 Proof.
   intros A n m o eq1 eq2 v.
   destruct eq1, eq2.
-  reflexivity.
+  repeat rewrite cast_rew; reflexivity.
 Qed.
 
-Theorem vector_length_coerce_id : forall {A n}
-    (eq : n = n) (v : Vector.t A n),
-    (vector_length_coerce eq v)
-    = v.
+Theorem cast_id : forall {A n} (eq : n = n) (v : t A n), (cast v eq) = v.
 Proof.
   intros A n eq v.
   replace eq with (eq_refl n).
-  - reflexivity.
+  - rewrite cast_rew; reflexivity.
   - apply proof_irrelevance.
 Qed.
 
-Theorem vector_length_coerce_inv : forall {A n m}
-    (eq : n = m) (v : Vector.t A n),
-    (vector_length_coerce (eq_sym eq) (vector_length_coerce eq v)) = v.
-Proof.
-  intros A n m eq v.
-  destruct eq.
-  reflexivity.
-Qed.
-
-Theorem vector_length_coerce_inv2 : forall {A n m}
-  (eq : m = n) (v : Vector.t A n),
-  (vector_length_coerce eq (vector_length_coerce (eq_sym eq) v)) = v.
-Proof.
-  intros A n m eq v.
-  destruct eq.
-  reflexivity.
-Qed.
-
-Theorem vector_length_coerce_cons : forall {A n m}
-  (h : A) (vn : Vector.t A n) (eq : S n = S m),
-  vector_length_coerce eq (h :: vn)
-  = h :: vector_length_coerce (succ_inj _ _ eq) vn.
+Theorem cast_cons : forall {A n m}
+  (h : A) (vn : t A n) (eq : S n = S m),
+  cast (h :: vn)  eq
+  = h :: cast vn (succ_inj _ _ eq).
 Proof.
   intros A n m h vn eq.
   destruct (succ_inj n m eq).
   replace eq with (eq_refl (S n)).
   2: { apply proof_irrelevance. }
-  simpl; f_equal.
+  reflexivity.
 Qed.
 
-Theorem vector_length_coerce_app_l : forall {A n m o}
-  (vn : Vector.t A n) (vm : Vector.t A m) (eq : n + m = n + o),
-  vector_length_coerce eq (vn ++ vm)
-  = vn ++ vector_length_coerce (Plus.plus_reg_l _ _ _ eq) vm.
+Theorem cast_app_l : forall {A n m o}
+  (vn : t A n) (vm : t A m) (eq : n + m = n + o),
+  cast (vn ++ vm)  eq
+  = vn ++ cast vm (Plus.plus_reg_l _ _ _ eq).
 Proof.
   intros A n m o vn vm eq.
   destruct (Plus.plus_reg_l _ _ _ eq).
   replace eq with (eq_refl (n + m)).
   2: { apply proof_irrelevance. }
-  simpl; f_equal.
+  repeat rewrite cast_id; reflexivity.
 Qed.
 
-Theorem vector_length_coerce_app_r : forall {A n m o}
-  (vn : Vector.t A n) (vm : Vector.t A m) (eq : n + m = o + m),
-  vector_length_coerce eq (vn ++ vm)
-  = vector_length_coerce (plus_reg_r _ _ _ eq) vn ++ vm.
+Theorem cast_app_r : forall {A n m o}
+  (vn : t A n) (vm : t A m) (eq : n + m = o + m),
+  cast (vn ++ vm) eq
+  = cast vn (plus_reg_r _ _ _ eq) ++ vm.
 Proof.
   intros A n m o vn vm eq.
   destruct (plus_reg_r _ _ _ eq).
   replace eq with (eq_refl (n + m)).
   2: { apply proof_irrelevance. }
-  simpl; f_equal.
+  repeat rewrite cast_id; reflexivity.
 Qed.
 
-Theorem vector_length_coerce_app_funct : forall {A n1 n2 m1 m2}
+Theorem cast_app_funct : forall {A n1 n2 m1 m2}
   (neq : n1 = n2) (meq : m1 = m2)
-  (vn : Vector.t A n1) (vm : Vector.t A m1),
-  vector_length_coerce neq vn ++ vector_length_coerce meq vm
-  = vector_length_coerce (f_equal2_plus _ _ _ _ neq meq) (vn ++ vm).
+  (vn : t A n1) (vm : t A m1),
+  cast vn neq ++ cast vm meq
+  = cast (vn ++ vm) (f_equal2_plus _ _ _ _ neq meq).
 Proof.
   intros A n1 n2 m1 m2 neq meq vn vm.
   destruct neq, meq.
   replace (f_equal2_plus _ _ _ _ _ _) with (eq_refl (n1 + m1)).
-  { reflexivity. }
+  { repeat rewrite cast_id; reflexivity. }
   apply proof_irrelevance.
 Qed.
 
-Theorem vector_length_coerce_app_assoc_1 : forall {A n m o}
-  (vn : Vector.t A n) (vm : Vector.t A m) (vo : Vector.t A o),
-  vector_length_coerce (add_assoc n m o) (vn ++ (vm ++ vo))
+
+
+Theorem cast_app_right_lem :
+  forall n m o, m = o -> m + n = o + n.
+Proof. intros n m o eq; destruct eq; reflexivity. Qed.
+
+Theorem cast_app_right : 
+  forall {A n m o} (vn : t A n) (vm : t A m) (eq : m = o),
+    cast vm eq ++ vn = cast (vm ++ vn) (cast_app_right_lem n m o eq).
+Proof.
+  intros A n m o vn vm eq; destruct eq.
+  repeat rewrite cast_id.
+  reflexivity.
+Qed.
+
+Theorem cast_app_left_lem :
+  forall n m o, m = o -> n + m = n + o.
+Proof. intros n m o eq; destruct eq; reflexivity. Qed.
+
+Theorem cast_app_left : 
+  forall {A n m o} (vn : t A n) (vm : t A m) (eq : m = o),
+    vn ++ cast vm eq =
+    cast (vn ++ vm) (cast_app_left_lem n m o eq).
+Proof.
+  intros A n m o vn vm eq; destruct eq.
+  repeat rewrite cast_id.
+  reflexivity.
+Qed.
+
+Theorem cast_app_assoc_1 : forall {A n m o}
+  (vn : t A n) (vm : t A m) (vo : t A o),
+  cast (vn ++ (vm ++ vo)) (add_assoc n m o)
   = (vn ++ vm) ++ vo.
 Proof.
   intros A n m o vn vm vo.
   induction vn.
   - simpl.
     replace (add_assoc 0 m o) with (eq_refl (m + o)).
-    + reflexivity.
+    + rewrite cast_id; reflexivity.
     + apply proof_irrelevance.
   - simpl.
-    rewrite vector_length_coerce_cons.
     f_equal.
     rewrite <- IHvn.
     f_equal.
     apply proof_irrelevance.
 Qed.
 
-Theorem vector_length_coerce_app_assoc_2 : forall {A n m o}
-  (vn : Vector.t A n) (vm : Vector.t A m) (vo : Vector.t A o),
-  vector_length_coerce (eq_sym (add_assoc n m o)) ((vn ++ vm) ++ vo)
+Theorem cast_app_assoc_2 : forall {A n m o}
+  (vn : t A n) (vm : t A m) (vo : t A o),
+  cast ((vn ++ vm) ++ vo)  (eq_sym (add_assoc n m o))
   = vn ++ (vm ++ vo).
 Proof.
   intros A n m o vn vm vo.
   induction vn.
   - simpl.
     replace (add_assoc 0 m o) with (eq_refl (m + o)).
-    + reflexivity.
+    + rewrite cast_id; reflexivity.
     + apply proof_irrelevance.
   - simpl.
-    rewrite vector_length_coerce_cons.
     f_equal.
     rewrite <- IHvn.
     f_equal.
@@ -151,23 +161,22 @@ Proof.
 Qed.
 
 Definition vector_cons_split : forall {A n}
-  (v : Vector.t A (S n)), 
-  { x : A & { vtl : Vector.t A n | v = Vector.cons A x n vtl } }.
+  (v : t A (S n)), 
+  { x : A & { vtl : t A n | v = cons A x n vtl } }.
   intros A n v.
-  exists (Vector.hd v), (Vector.tl v). apply Vector.eta.
+  exists (hd v), (tl v). apply Vector.eta.
 Defined.
 
-
 Definition replace :
-  forall {A n} (v : Vector.t A n) (p: fin n) (a : A), Vector.t A n.
+  forall {A n} (v : t A n) (p: fin n) (a : A), t A n.
   intros A n; induction n as [|n IHn]; intros v [p pprp] a.
-  - apply Vector.nil.
+  - apply nil.
   - destruct (vector_cons_split v) as [vhd [vtl _]].
     destruct p.
-    + apply Vector.cons.
+    + apply cons.
       * exact a.
       * exact vtl.
-    + apply Vector.cons.
+    + apply cons.
       * exact vhd.
       * apply (fun x => IHn vtl x a).
         exists p.
@@ -175,7 +184,7 @@ Definition replace :
 Defined. 
 
 Definition nth :
-  forall {A n} (v : Vector.t A n) (p: fin n), A.
+  forall {A n} (v : t A n) (p: fin n), A.
   intros A n; induction n as [|n IHn]; intros v [p pprp].
   - destruct (nlt_0_r _ pprp).
   - destruct (vector_cons_split v) as [vhd [vtl _]].
@@ -187,7 +196,7 @@ Definition nth :
 Defined.
 
 Theorem vector_rev_append_nil_o : forall {A n}
-  (v : Vector.t A n),
+  (v : t A n),
   rev_append [] v = v.
 Proof.
   intros A n v.
@@ -204,16 +213,16 @@ Proof.
 Qed.
 
 Theorem rev_coerce_unfold : forall {A n}
-  (v : Vector.t A n),
+  (v : t A n),
   rev v = 
-  vector_length_coerce (eq_sym (plus_n_O n))
-    (rev_append v []).
+  cast (rev_append v []) (eq_sym (plus_n_O n)).
 Proof.
-  reflexivity.
+  intros A n v.
+  rewrite cast_rew; reflexivity.
 Qed.
 
 Theorem vector_rev_nil_nil : forall {A},
-  rev [] = ([] : Vector.t A 0).
+  rev [] = ([] : t A 0).
 Proof.
   intros A.
   rewrite rev_coerce_unfold.
@@ -246,8 +255,8 @@ Defined.
 Definition most : forall {A n}, t A (S n) -> t A n.
   intros A n v.
   induction n.
-  - apply Vector.nil.
-  - apply Vector.cons.
+  - apply nil.
+  - apply cons.
     + exact (hd v).
     + apply IHn.
       exact (tl v).
@@ -260,9 +269,8 @@ Definition most_ : forall {A n}, t A (n + 1) -> t A n.
   exact v.
 Defined.
 
-  
 Theorem vector_snoc_eta : forall {A n}
-  (v : Vector.t A (n + 1)),
+  (v : t A (n + 1)),
   v = most_ v ++ [last_ v].
 Proof.
   intros A n v.
@@ -280,82 +288,55 @@ Proof.
     { apply IHn. }
     rewrite H at 1.
     simpl; f_equal.
-    + change (eq_rect _ _ _ _ _)
-        with (vector_length_coerce (add_comm (S n) 1) (hd v :: tl v)).
-      rewrite (vector_length_coerce_cons _ (tl v)).
+    + rewrite <- cast_rew.
       reflexivity.
     + f_equal.
-      * change (eq_rect _ _ _ _ _)
-          with (vector_length_coerce (add_comm (S n) 1) (hd v :: tl v)).
-        rewrite (vector_length_coerce_cons _ (tl v)).
+      * rewrite <- cast_rew.
         simpl; unfold most_.
-        unfold vector_length_coerce.
+        rewrite cast_rew.
         repeat f_equal.
         apply proof_irrelevance.
       * unfold last_ at 2.
-        change (eq_rect _ _ _ _ _)
-          with (vector_length_coerce (add_comm (S n) 1) (hd v :: tl v)).
-        rewrite (vector_length_coerce_cons _ (tl v)).
-        unfold last_, vector_length_coerce.
+        rewrite <- cast_rew.
+        rewrite (cast_cons _ (tl v)).
+        unfold last_; rewrite cast_rew.
         simpl; repeat f_equal.
         apply proof_irrelevance.
 Qed.
 
-Theorem depEqLem : 
-  forall (B : Type) 
-         (F : B -> Type)
-         (P : forall b : B, F b -> Prop)
-         (b1 b2 : B) (eqb : b1 = b2)
-         (p1 : F b1) (p2 : F b2),
-         (rew eqb in p1 = p2) ->
-         P b1 p1 ->
-         P b2 p2.
-Proof.
-  intros B F P b1 b2 eqb.
-  destruct eqb.
-  intros p1 p2 eqp.
-  destruct eqp.
-  intros Pp.
-  exact Pp.
-Qed.         
 
 Theorem t_snoc_ind : forall (A : Type) (P : forall n : nat, t A n -> Prop),
   P 0 [] ->
-  (forall (h : A) (n : nat) (t : t A n), P n t -> P (n + 1) (t ++ [h])) ->
-  forall (n : nat) (t : t A n), P n t.
+  (forall (h : A) (n : nat) (v : t A n), P n v -> P (n + 1) (v ++ [h])) ->
+  forall (n : nat) (v : t A n), P n v.
 Proof.
-  intros A P Pnil Psnoc n t.
+  intros A P Pnil Psnoc n v.
   induction n.
-  - rewrite (vector_nil_eq t).
+  - rewrite (vector_nil_eq v).
     exact Pnil.
-  - remember (vector_length_coerce (eq_sym (add_comm n 1)) t) as t'.
-    assert (t' = most_ t' ++ [last_ t']).
+  - remember (cast v (eq_sym (add_comm n 1))) as v'.
+    assert (v' = most_ v' ++ [last_ v']).
     { apply vector_snoc_eta. }
-    assert (P n (most_ t')).
+    assert (P n (most_ v')).
     { apply IHn. }
-    apply (Psnoc (last_ t') _ _) in H0.
+    apply (Psnoc (last_ v') _ _) in H0.
     assert (n + 1 = S n).
     { rewrite add_comm; reflexivity. }
-    apply (depEqLem nat (Vector.t A) P (n + 1) (S n) H1 t' t).
+    apply (depEqLem nat (t A) P (n + 1) (S n) H1 v' v).
     2: { rewrite H; assumption. }
-    rewrite Heqt'.
-    unfold vector_length_coerce.
-    rewrite rew_compose.
-    replace (Logic.eq_trans (eq_sym (add_comm n 1)) H1) with (eq_refl (S n)).
-    + reflexivity.
-    + apply proof_irrelevance.
+    rewrite Heqv', cast_rew, rew_compose, rew_id.
+    reflexivity.
 Qed.
 
 Theorem rev_append_step : forall {A n m}
-  (h : A) (vn : Vector.t A n) (vm : Vector.t A m),
+  (h : A) (vn : t A n) (vm : t A m),
   rev_append (h :: vn) vm =
-  vector_length_coerce (eq_sym (plus_n_Sm n m))
-    (rev_append vn (h :: vm)).
+  cast (rev_append vn (h :: vm)) (eq_sym (plus_n_Sm n m)).
 Proof.
   intros A n m h vn vm.
   unfold rev_append.
   simpl rev_append_tail.
-  unfold vector_length_coerce.
+  rewrite cast_rew.
   unfold eq_rect_r.
   rewrite rew_compose.
   f_equal.
@@ -363,15 +344,14 @@ Proof.
 Qed.
 
 Theorem rev_append_unstep : forall {A n m}
-  (h : A) (vn : Vector.t A n) (vm : Vector.t A m),
+  (h : A) (vn : t A n) (vm : t A m),
   rev_append vn (h :: vm) =
-  vector_length_coerce (plus_n_Sm n m)
-    (rev_append (h :: vn) vm).
+  cast (rev_append (h :: vn) vm) (plus_n_Sm n m).
 Proof.
   intros A n m h vn vm.
   unfold rev_append.
   simpl rev_append_tail.
-  unfold vector_length_coerce.
+  rewrite cast_rew.
   unfold eq_rect_r.
   rewrite rew_compose.
   f_equal.
@@ -379,24 +359,23 @@ Proof.
 Qed.
 
 Theorem append_nil : forall {A n}
-  (vn : Vector.t A n),
+  (vn : t A n),
   vn ++ [] =
-  vector_length_coerce (plus_n_O n) vn.
+  cast vn (plus_n_O n).
 Proof.
   intros A n vn; induction vn.
-  - rewrite vector_length_coerce_id.
+  - rewrite cast_id.
     reflexivity.
   - simpl.
     rewrite IHvn.
-    rewrite vector_length_coerce_cons.
     repeat f_equal.
     apply proof_irrelevance.
 Qed.
 
-Theorem vector_length_coerce_cons_in : forall {A n m}
-  (eq : n = m) (h : A) (vn : Vector.t A n),
-  h :: vector_length_coerce eq vn
-  = vector_length_coerce (eq_S _ _ eq) (h :: vn).
+Theorem cast_cons_in : forall {A n m}
+  (eq : n = m) (h : A) (vn : t A n),
+  h :: cast vn eq
+  = cast (h :: vn) (eq_S _ _ eq).
 Proof.
   intros A n m eq h vn.
   destruct eq.
@@ -408,11 +387,9 @@ Theorem rev_append_app_step_lem : forall {n m},
 Proof. lia. Qed.
 
 Theorem rev_append_cons : forall {A n m}
-  (h : A) (vn : Vector.t A n) (vm : Vector.t A m),
+  (h : A) (vn : t A n) (vm : t A m),
   rev_append (vn ++ [h]) vm =
-  vector_length_coerce
-    rev_append_app_step_lem
-    (h :: rev_append vn vm).
+  cast (h :: rev_append vn vm) rev_append_app_step_lem.
 Proof.
   intros A n m h vn vm.
   generalize dependent m.
@@ -422,114 +399,107 @@ Proof.
     replace (rev_append [h] vm)
        with (rev_append [] (h :: vm)).
     repeat rewrite vector_rev_append_nil_o.
-    rewrite vector_length_coerce_id.
+    rewrite cast_id.
     reflexivity.
     rewrite rev_append_step.
-    rewrite vector_length_coerce_id.
+    rewrite cast_id.
     reflexivity.
   - simpl. 
     rewrite rev_append_step.
     rewrite IHvn.
     rewrite rev_append_step.
-    rewrite vector_length_coerce_cons_in.
-    repeat rewrite vector_length_coerce_trans.
+    repeat rewrite cast_cons_in, cast_trans.
     f_equal; apply proof_irrelevance.
 Qed.
 
 Theorem rev_append_app : forall {A n m o}
-  (vn : Vector.t A n) (vm : Vector.t A m) (vo : Vector.t A o),
+  (vn : t A n) (vm : t A m) (vo : t A o),
   rev_append vn vm ++ vo =
-  vector_length_coerce (add_assoc n m o)
-    (rev_append vn (vm ++ vo)).
+  cast (rev_append vn (vm ++ vo)) (add_assoc n m o).
 Proof.
   intros A n m o vn vm vo.
   generalize dependent m.
   generalize dependent o.
   induction vn; intros.
   - repeat rewrite vector_rev_append_nil_o.
-    rewrite vector_length_coerce_id.
+    rewrite cast_id.
     reflexivity.
   - repeat rewrite rev_append_step.
-    rewrite <- (vector_length_coerce_id (eq_refl o) vo) at 1.
-    rewrite vector_length_coerce_app_funct.
+    rewrite <- (cast_id (eq_refl o) vo) at 1.
+    rewrite cast_app_funct.
     rewrite (IHvn _ vo _ (h :: vm)).
-    repeat rewrite vector_length_coerce_trans.
+    repeat rewrite cast_trans.
     f_equal.
     apply proof_irrelevance.
 Qed.
 
 Theorem rev_append_app_2 : forall {A n m o}
-  (vn : Vector.t A n) (vm : Vector.t A m) (vo : Vector.t A o),
+  (vn : t A n) (vm : t A m) (vo : t A o),
   rev_append vn (vm ++ vo) =
-  vector_length_coerce (eq_sym (add_assoc n m o))
-    (rev_append vn vm ++ vo).
+  cast (rev_append vn vm ++ vo) (eq_sym (add_assoc n m o)).
 Proof.
   intros A n m o vn vm vo.
   rewrite rev_append_app.
-  rewrite vector_length_coerce_trans.
-  rewrite vector_length_coerce_id.
+  rewrite cast_trans.
+  rewrite cast_id.
   reflexivity.
 Qed.
 
-Theorem rev_cons : forall {A n} (h : A) (v : Vector.t A n),
-  rev (v ++ [h]) = 
-  vector_length_coerce (add_comm 1 n) (h :: rev v).
+Theorem rev_cons : forall {A n} (h : A) (v : t A n),
+  rev (v ++ [h]) = cast (h :: rev v)  (add_comm 1 n).
 Proof.
   intros A n h v.
   repeat rewrite rev_coerce_unfold.
   rewrite rev_append_cons.
-  rewrite vector_length_coerce_cons_in.
-  repeat rewrite vector_length_coerce_trans.
+  rewrite cast_cons_in.
+  repeat rewrite cast_trans.
   f_equal.
   apply proof_irrelevance.
 Qed.
 
-Theorem rev_snoc : forall {A n} (h : A) (v : Vector.t A n),
-  rev (h :: v) = 
-  vector_length_coerce (add_comm n 1) (rev v ++ [h]).
+Theorem rev_snoc : forall {A n} (h : A) (v : t A n),
+  rev (h :: v) = cast (rev v ++ [h]) (add_comm n 1).
 Proof.
   intros A n h v.
   repeat rewrite rev_coerce_unfold.
-  rewrite rev_append_step.
-  rewrite <- (vector_length_coerce_id (eq_refl 1) [h]) at 2.
-  rewrite vector_length_coerce_app_funct.
+  rewrite rev_append_step, cast_app_right.
   rewrite (rev_append_app v [] [h]).
-  simpl.
-  repeat rewrite vector_length_coerce_trans.
+  repeat rewrite cast_trans.
   f_equal.
   apply proof_irrelevance.
 Qed.
 
-Theorem vector_length_coerce_f_swap : forall {A n m}
+Theorem cast_f_swap : forall {A n m}
   (f : forall x, t A x -> t A x)
   (eq : n = m)
   (v : t A n),
-  f _ (vector_length_coerce eq v) =
-  vector_length_coerce eq (f _ v).
+  f _ (cast v eq) =
+  cast (f _ v) eq.
 Proof.
-  intros A n m f eq.
-  destruct eq.
+  intros A n m f eq v.
+  destruct eq. 
+  repeat rewrite cast_id.
   reflexivity.
 Qed.
 
 Theorem vector_rev_rev_id : forall {A n}
-  (v : Vector.t A n),
+  (v : t A n),
   rev (rev v) = v.
 Proof.
   intros A n v; induction v using t_snoc_ind.
   - repeat rewrite vector_rev_nil_nil.
     reflexivity.
   - rewrite rev_cons.
-    rewrite (vector_length_coerce_f_swap (@rev A)).
+    rewrite (cast_f_swap (@rev A)).
     rewrite rev_snoc, IHv,
-            vector_length_coerce_trans,
-            vector_length_coerce_id.
+            cast_trans,
+            cast_id.
     reflexivity.
 Qed.
 
 Theorem vector_append_inv1 : forall {A n m}
-    (v : Vector.t A (n + m)),
-    uncurry Vector.append (Vector.splitat _ v) = v.
+    (v : t A (n + m)),
+    uncurry append (splitat _ v) = v.
 Proof.
   intros A n.
   induction n as [|n IHn];
@@ -539,17 +509,17 @@ Proof.
     simpl in v.
     destruct (vector_cons_split v) as [x [vtl eq]].
     rewrite eq.
-    assert (uncurry Vector.append (Vector.splitat n vtl) = vtl).
+    assert (uncurry append (splitat n vtl) = vtl).
     { apply IHn. }
     simpl.
-    destruct (Vector.splitat n vtl) as [tl1 tl2].
+    destruct (splitat n vtl) as [tl1 tl2].
     rewrite <- H.
     reflexivity.
 Qed.
 
 Theorem vector_append_inv2 : forall {A n m}
-    (v1 : Vector.t A n) (v2 : Vector.t A m),
-    Vector.splitat _ (Vector.append v1 v2) = (v1, v2).
+    (v1 : t A n) (v2 : t A m),
+    splitat _ (append v1 v2) = (v1, v2).
   intros A n m v.
   generalize dependent m.
   induction v.
@@ -561,66 +531,66 @@ Theorem vector_append_inv2 : forall {A n m}
 Qed.
 
 Theorem vector_append_split : forall {A n m}
-  (v : Vector.t A (n + m)), 
-  (exists (vhd : Vector.t A n) (vtl : Vector.t A m),
-  v = Vector.append vhd vtl).
+  (v : t A (n + m)), 
+  (exists (vhd : t A n) (vtl : t A m),
+  v = append vhd vtl).
 Proof.
   intros A n m v.
   rewrite <- (vector_append_inv1 v).
-  destruct (Vector.splitat n v) as [v1 v2].
+  destruct (splitat n v) as [v1 v2].
   exists v1, v2.
   reflexivity.
 Qed.
 
 Definition vector_concat : forall {A n m},
-    Vector.t (Vector.t A n) m -> Vector.t A (m * n).
+    t (t A n) m -> t A (m * n).
   intros A n m v.
   induction v.
-  - apply Vector.nil.
+  - apply nil.
   - simpl.
-    apply Vector.append.
+    apply append.
     + apply h.
     + apply IHv.
 Defined.
 
 Definition vector_unconcat : forall {A n m},
-    Vector.t A (m * n) -> Vector.t (Vector.t A n) m.
+    t A (m * n) -> t (t A n) m.
   intros A n m v.
   induction m as [|m IHm].
-  - apply Vector.nil.
-  - simpl in v; destruct (Vector.splitat _ v) as [vv1 vvtl].
-    apply Vector.cons.
+  - apply nil.
+  - simpl in v; destruct (splitat _ v) as [vv1 vvtl].
+    apply cons.
     + apply vv1.
     + apply IHm.
       apply vvtl.
 Defined.
 
 Theorem vector_concat_inv1_lem : forall {A n m}
-  (v : Vector.t A (n * m))
-  (u : Vector.t A m),
-  vector_unconcat (Vector.append u v : Vector.t A (S n * m)) =
-  Vector.cons _ u _ (vector_unconcat v).
+  (v : t A (n * m))
+  (u : t A m),
+  vector_unconcat (append u v : t A (S n * m)) =
+  cons _ u _ (vector_unconcat v).
 Proof.
   intros A n m v u.
   generalize dependent v.
   induction u.
   - reflexivity.
   - intros v.
-    simpl Vector.append.
+    simpl append.
     simpl vector_unconcat.
     rewrite vector_append_inv2.
     reflexivity.
 Qed.
 
 Theorem vector_concat_inv1 : forall {A n m}
-  (v : Vector.t A (n * m)),
+  (v : t A (n * m)),
   vector_concat (vector_unconcat v) = v.
 Proof.
   intros A n.
   induction n as [|n IHn];
   intros m v.
   - simpl.
-    apply (Vector.case0 (fun v => Vector.nil A = v)).
+    apply (case0 (fun v => nil A = v)).
     reflexivity.
   - simpl in v.
     destruct (vector_append_split v) as [vhd [vtl eq]].
@@ -632,7 +602,7 @@ Proof.
 Qed.
 
 Theorem vector_concat_inv2 : forall {A n m}
-    (v : Vector.t (Vector.t A n) m),
+    (v : t (t A n) m),
     vector_unconcat (vector_concat v) = v.
   intros A n m.
   induction v.
@@ -644,9 +614,9 @@ Theorem vector_concat_inv2 : forall {A n m}
 Qed.
 
 Definition vector_concat_2 : forall {A n m},
-    Vector.t (Vector.t A n) m -> Vector.t A (n * m).
+    t (t A n) m -> t A (n * m).
   intros A n m v.
-  rewrite PeanoNat.Nat.mul_comm.
+  rewrite mul_comm.
   apply vector_concat.
   assumption.
 Defined.
@@ -686,113 +656,81 @@ Definition Block_Lem : forall idx blksz memsz,
 Defined.
 
 Definition Block_Load_Store : forall {B memsz}
-    (m : Vector.t B memsz)
+    (m : t B memsz)
     (idx blksz: fin memsz)
-    (block : Vector.t B (proj1_sig blksz)),
-    Vector.t B (proj1_sig blksz) * Vector.t B memsz.
+    (block : t B (proj1_sig blksz)),
+    t B (proj1_sig blksz) * t B memsz.
   intros B memsz m [idx lip] [blksz lbp] block.
   destruct (Block_Lem _ _ _ lip lbp) as 
     [[tl eq]|[blk1[blk2[idx2[eq1 [eq2 eq3]]]]]].
   - rewrite eq in m.
-    destruct (Vector.splitat _ m) as [m' m3].
-    destruct (Vector.splitat _ m') as [m1 m2].
+    destruct (splitat _ m) as [m' m3].
+    destruct (splitat _ m') as [m1 m2].
     split.
     { exact m2. }
     rewrite eq.
-    exact (Vector.append (Vector.append m1 block) m3).
+    exact (append (append m1 block) m3).
   - rewrite eq3 in m.
-    destruct (Vector.splitat _ m) as [m' m3].
-    destruct (Vector.splitat _ m') as [m1 m2].
+    destruct (splitat _ m) as [m' m3].
+    destruct (splitat _ m') as [m1 m2].
     split.
-    + apply (vector_length_coerce eq1).
+    + apply (fun x => cast x eq1).
       (* Note: m1 is an overflow, so it's
               bits are more significant than m3. *)
       rewrite add_comm.
-      apply (Vector.append m3 m1).
+      apply (append m3 m1).
     + rewrite <- eq1 in block.
-      destruct (Vector.splitat _ block) as [block1 block2].
+      destruct (splitat _ block) as [block1 block2].
       rewrite eq3.
       (* Note: The overflow means block2 should go at
               the begining of memory, and block 1 at the end. *)
       assert (blk1 + idx2 + blk2 = blk2 + idx2 + blk1) as OvrEq.
       { lia. }
       rewrite OvrEq.
-      exact (Vector.append (Vector.append block2 m2) block1).
+      exact (append (append block2 m2) block1).
 Defined.
 
 (* Memory_Block_Load w/o rebuilding memory. *)
 Definition Block_Load : forall {B memsz}
-    (m : Vector.t B memsz)
+    (m : t B memsz)
     (idx blksz: fin memsz),
-    Vector.t B (proj1_sig blksz).
+    t B (proj1_sig blksz).
   intros B memsz m [idx lip] [blksz lbp].
   destruct (Block_Lem _ _ _ lip lbp) as 
     [[tl eq]|[blk1[blk2[idx2[eq1 [eq2 eq3]]]]]].
   - rewrite eq in m.
-    destruct (Vector.splitat _ m) as [m' _].
-    destruct (Vector.splitat _ m') as [_ m2].
+    destruct (splitat _ m) as [m' _].
+    destruct (splitat _ m') as [_ m2].
     exact m2.
   - rewrite eq3 in m.
-    destruct (Vector.splitat _ m) as [m' m3].
-    destruct (Vector.splitat _ m') as [m1 _].
-    apply (vector_length_coerce eq1).
+    destruct (splitat _ m) as [m' m3].
+    destruct (splitat _ m') as [m1 _].
+    apply (fun x => cast x eq1).
     (* Note: m1 is an overflow, so it's
               bits are more significant than m3. *)
     rewrite add_comm.
-    apply (Vector.append m3 m1).
+    apply (append m3 m1).
 Defined.
 
 Definition Block_Store {B memsz}
-    (m : Vector.t B memsz)
+    (m : t B memsz)
     (idx blksz: fin memsz)
-    (block : Vector.t B (proj1_sig blksz)) :
-    Vector.t B memsz :=
+    (block : t B (proj1_sig blksz)) :
+    t B memsz :=
   snd (Block_Load_Store m idx blksz block).
-
-Theorem vector_length_coerce_app_right_lem :
-  forall n m o, m = o -> m + n = o + n.
-Proof.
-  intros n m o eq; destruct eq; reflexivity.
-Qed.
-
-Theorem vector_length_coerce_app_right : 
-  forall {A n m o} (vn : Vector.t A n) (vm : Vector.t A m) (eq : m = o),
-    vector_length_coerce eq vm ++ vn =
-    vector_length_coerce (vector_length_coerce_app_right_lem n m o eq) (vm ++ vn).
-Proof.
-  intros A n m o vn vm eq; destruct eq.
-  repeat rewrite vector_length_coerce_id.
-  reflexivity.
-Qed.
-
-Theorem vector_length_coerce_app_left_lem :
-  forall n m o, m = o -> n + m = n + o.
-Proof.
-  intros n m o eq; destruct eq; reflexivity.
-Qed.
-
-Theorem vector_length_coerce_app_left : 
-  forall {A n m o} (vn : Vector.t A n) (vm : Vector.t A m) (eq : m = o),
-    vn ++ vector_length_coerce eq vm =
-    vector_length_coerce (vector_length_coerce_app_left_lem n m o eq) (vn ++ vm).
-Proof.
-  intros A n m o vn vm eq; destruct eq.
-  repeat rewrite vector_length_coerce_id.
-  reflexivity.
-Qed.
 
 Ltac vector_bubble :=
   match goal with
-  | |- context[vector_length_coerce _ (vector_length_coerce _ _)] =>
-      rewrite vector_length_coerce_trans
-  | |- context[?x ++ vector_length_coerce _ ?y] =>
-      rewrite vector_length_coerce_app_left
-  | |- context[vector_length_coerce _ ?x ++ ?y] =>
-      rewrite vector_length_coerce_app_right
-  | |- context[?h :: vector_length_coerce _ ?y] =>
-      rewrite vector_length_coerce_cons_in
+  | |- context[cast _ (cast _ _)] =>
+      rewrite cast_trans
+  | |- context[?x ++ cast _ ?y] =>
+      rewrite cast_app_left
+  | |- context[cast _ ?x ++ ?y] =>
+      rewrite cast_app_right
+  | |- context[?h :: cast _ ?y] =>
+      rewrite cast_cons_in
   | |- context[(?vn ++ ?vm) ++ ?vo] =>
-      rewrite <- vector_length_coerce_app_assoc_1
+      rewrite <- cast_app_assoc_1
   | |- context[rev []] =>
       rewrite vector_rev_nil_nil
   | |- context[rev (rev ?x)] =>
@@ -805,7 +743,7 @@ Ltac vector_bubble :=
 
 Ltac vector_simp :=
   repeat vector_bubble;
-  repeat rewrite vector_length_coerce_id.
+  repeat rewrite cast_id.
 
 Example test : rev [false ; false ; false ; false ; false ]
                  = [ false ; false ; false ; false ; false ].
